src/Init/Data/Array/Lemmas.lean
@@ -961,6 +961,27 @@ theorem get_append_right {as bs : Array α} {h : i < (as ++ bs).size} (hle : as.
 theorem append_assoc (as bs cs : Array α) : as ++ bs ++ cs = as ++ (bs ++ cs) := by
   apply ext'; simp only [append_toList, List.append_assoc]
 
+/-! ### join -/
+
+@[simp] theorem toList_join {l : Array (Array α)} : l.join.toList = (l.toList.map toList).join := by
+  dsimp [join]
+  simp only [foldl_eq_foldl_toList]
+  generalize l.toList = l
+  have : ∀ a : Array α, (List.foldl ?_ a l).toList = a.toList ++ ?_ := ?_
+  exact this #[]
+  induction l with
+  | nil => simp
+  | cons h => induction h.toList <;> simp [*]
+
+theorem mem_join : ∀ {L : Array (Array α)}, a ∈ L.join ↔ ∃ l, l ∈ L ∧ a ∈ l := by
+  simp only [mem_def, toList_join, List.mem_join, List.mem_map]
+  intro l
+  constructor
+  · rintro ⟨_, ⟨s, m, rfl⟩, h⟩
+    exact ⟨s, m, h⟩
+  · rintro ⟨s, h₁, h₂⟩
+    refine ⟨s.toList, ⟨⟨s, h₁, rfl⟩, h₂⟩⟩
+
 /-! ### extract -/
 
 theorem extract_loop_zero (as bs : Array α) (start : Nat) : extract.loop as 0 start bs = bs := by
@@ -1381,6 +1402,10 @@ Our goal is to have `simp` "pull `List.toArray` outwards" as much as possible.
     l₁.toArray ++ l₂.toArray = (l₁ ++ l₂).toArray := by
   apply ext'
   simp
+
+@[simp] theorem join_toArray (l : List (List α)) : (l.toArray.map List.toArray).join = l.join.toArray := by
+  apply ext'
+  simp [Function.comp_def]
 
 @[simp] theorem toArray_range (n : Nat) : (range n).toArray = Array.range n := by
   apply ext'
